Projects/Esolangs/Cornucopia/Programs.lean
@@ -1,0 +1,5 @@
+import Projects.Esolangs.Cornucopia.Programs.Id
+import Projects.Esolangs.Cornucopia.Programs.Loop
+import Projects.Esolangs.Cornucopia.Programs.LoopSucc1
+import Projects.Esolangs.Cornucopia.Programs.LoopSucc2
+import Projects.Esolangs.Cornucopia.Programs.Prog1
