Projects/Esolangs/Cornucopia/Programs/Id.lean
@@ -1,0 +1,74 @@
+import Projects.Esolangs.Cornucopia.Basic
+
+attribute [-simp] List.getElem!_eq_getElem?_getD
+
+namespace Esolangs.Cornucopia.Programs.Id
+
+def exprId : Expr :=
+  .arg 0
+
+def defs : List (String × Def) :=
+  [(mainName, ⟨1, exprId⟩)]
+
+def fs : Map String (List ℕ → ℕ) :=
+  .ofList [(mainName, fn 1 (·[0]!))]
+
+def prog : Prog :=
+  .ofDefs defs
+
+-----
+
+@[simp]
+theorem nodup_defs : defs.map (·.1) |>.Nodup := by
+  simp [defs]
+
+@[simp]
+theorem wfDefs' : WFDefs' defs := by
+  constructor <;> simp [defs, exprId]
+
+@[instance, simp]
+theorem wf' : prog.WF' :=
+  wfDefs'.wf'
+
+@[simp]
+theorem compatibleDefs : CompatibleDefs (.ofList defs) fs := by
+  use by simp [defs, fs]
+  intro name d; simp [defs, fs, Map.get?_insert]
+  rintro rfl rfl; simp [exprId]
+
+@[simp]
+theorem compatible : prog.Compatible (builtinFs ∪ fs) :=
+  wfDefs'.compatible compatibleDefs
+
+@[instance, simp]
+theorem wf_prog : prog.WF := by
+  apply wfDefs'.wf; use fs, compatibleDefs
+  intro fs' h₁ name d f h₂ h₃
+  simp [fs, Map.get!_insert]
+  have h₅ := h₁.eval_eq h₂ |>.symm
+  simp [h₃] at h₅
+  subst h₅
+  simp [funext_iff, fn]
+  intro xs
+  simp [defs] at h₂
+  rcases h₂ with ⟨rfl, rfl⟩
+  simp [fn, exprId]
+
+@[simp]
+theorem fs_prog : prog.fs = builtinFs ∪ fs :=
+  prog.fs_eq_of_compatible compatible
+
+@[simp]
+theorem run_prog {n} : prog.run n = n := by
+  simp [Prog.run, Prog.eval, fs, Map.get!_insert, fn]
+
+instance : ProgInfo prog where
+  name := "Id"
+  defNames := ["main"]
+  has_model := true
+  has_unique_model := true
+  h_defNames := by
+    simp [prog, defs, builtinDefs, builtins, Map.ofList_eq_foldl, Map.keys_insert]; decide
+  h_wf' := by simp
+  h_has_model := by simp [Prog.HasModel]; use prog.fs; simp
+  h_has_unique_model := by simp [Prog.HasUniqueModel]; exact wf_prog.exiu_compatible
