Projects/Esolangs/Cornucopia/Programs/LoopSucc1.lean
@@ -1,0 +1,46 @@
+import Projects.Esolangs.Cornucopia.Basic
+
+attribute [-simp] List.getElem!_eq_getElem?_getD
+
+namespace Esolangs.Cornucopia.Programs.LoopSucc₁
+
+def exprLoopSucc (name : String) : Expr :=
+  .call succName [.call name [.arg 0]]
+
+def defs : List (String × Def) :=
+  [(mainName, ⟨1, exprLoopSucc mainName⟩)]
+
+def prog : Prog :=
+  .ofDefs defs
+
+-----
+
+@[simp]
+theorem nodup_defs : defs.map (·.1) |>.Nodup := by
+  simp [defs]
+
+@[simp]
+theorem wfDefs' : WFDefs' defs := by
+  constructor <;> simp [defs, exprLoopSucc]
+  simp [Prog.ofDefs, Map.get!_insert]
+
+@[instance, simp]
+theorem wf' : prog.WF' :=
+  wfDefs'.wf'
+
+@[instance, simp]
+theorem wfWoutModel_prog : prog.WFWoutModel := by
+  constructor; intro fs H
+  have h₁ := @H.eval_eq mainName (by simp) [0] (by simp)
+  simp [prog, defs, Prog.ofDefs, Map.get!_insert, exprLoopSucc, H.get!_builtin, fn] at h₁
+
+instance : ProgInfo prog where
+  name := "LoopSucc₁"
+  defNames := ["main"]
+  has_model := false
+  has_unique_model := false
+  h_defNames := by
+    simp [prog, defs, builtinDefs, builtins, Map.ofList_eq_foldl, Map.keys_insert]; decide
+  h_wf' := by simp
+  h_has_model := by simp [Prog.HasModel, wfWoutModel_prog.not_compatible]
+  h_has_unique_model := by simp [Prog.HasUniqueModel, wfWoutModel_prog.not_compatible]
