Projects/Esolangs/Cornucopia/Programs/LoopSucc2.lean
@@ -1,0 +1,69 @@
+import Projects.Esolangs.Cornucopia.Basic
+
+attribute [-simp] List.getElem!_eq_getElem?_getD
+
+namespace Esolangs.Cornucopia.Programs.LoopSucc₂
+
+def exprLoop (name : String) : Expr :=
+  .call name [.call succName [.arg 0]]
+
+def defs : List (String × Def) :=
+  [(mainName, ⟨1, exprLoop mainName⟩)]
+
+def fs (n : ℕ) : Map String (List ℕ → ℕ) :=
+  .ofList [(mainName, fn 1 # λ _ => n)]
+
+def prog : Prog :=
+  .ofDefs defs
+
+-----
+
+@[simp]
+theorem nodup_defs : defs.map (·.1) |>.Nodup := by
+  simp [defs]
+
+@[simp]
+theorem wfDefs' : WFDefs' defs := by
+  constructor <;> simp [defs, exprLoop]
+  simp [Prog.ofDefs, Map.get!_insert]
+
+@[instance, simp]
+theorem wf' : prog.WF' :=
+  wfDefs'.wf'
+
+@[simp]
+theorem compatibleDefs {n} : CompatibleDefs (.ofList defs) (fs n) := by
+  use by simp [defs, fs]
+  intro name d; simp [defs, fs, Map.get?_insert]
+  rintro rfl rfl; simp [exprLoop, Map.get!_insert, fn]
+
+@[simp]
+theorem compatible {n} : prog.Compatible (builtinFs ∪ fs n) :=
+  wfDefs'.compatible compatibleDefs
+
+@[simp]
+theorem builtin_not_mem_fs {n} {b : Builtin} : b.name ∉ fs n := by
+  simp [fs]
+
+@[simp]
+theorem fs_eq_fs_iff {n m} : fs n = fs m ↔ n = m := by
+  symm; use by grind;; simp [fs]; exact λ h => h [0] rfl
+
+@[instance, simp]
+theorem wfWoutUnique_prog : prog.WFWoutUnique := by
+  constructor
+  use builtinFs ∪ fs 0, builtinFs ∪ fs 1
+  simp [Map.union_eq_union_iff_right]
+
+instance : ProgInfo prog where
+  name := "Loop"
+  defNames := ["main"]
+  has_model := true
+  has_unique_model := false
+  h_defNames := by
+    simp [prog, defs, builtinDefs, builtins, Map.ofList_eq_foldl, Map.keys_insert]; decide
+  h_wf' := by simp
+  h_has_model := by
+    simp [Prog.HasModel]; use prog.fs; apply τ_spec; use builtinFs ∪ fs 0; simp
+  h_has_unique_model := by
+    have := wfWoutUnique_prog.exi_two; simp [Prog.HasUniqueModel, not_exiu_iff_or]; tauto
