Projects/Esolangs/Cornucopia/Show.lean
@@ -1,0 +1,43 @@
+import Projects.Esolangs.Cornucopia.Defs
+
+namespace Esolangs.Cornucopia
+
+def Prog.HasModel (prog : Prog) : Prop :=
+  ∃ fs, prog.Compatible fs
+
+def Prog.HasUniqueModel (prog : Prog) : Prop :=
+  ∃! fs, prog.Compatible fs
+
+class ProgInfo (prog : Prog) : Type where
+  name : String
+  defNames : List String
+  has_model : Bool
+  has_unique_model : Bool
+  h_defNames : prog.defs.keys.Perm # builtins.map Builtin.name ++ defNames
+  h_wf' : prog.WF'
+  h_has_model : prog.HasModel ↔ has_model
+  h_has_unique_model : prog.HasUniqueModel ↔ has_unique_model
+
+def Expr.show (e : Expr) (argNames : Array String) : String :=
+  match e with
+  | .arg i => argNames[i]!
+  | .call t args =>
+    t ++ if args.length = 0 then "" else
+    "(" ++ ", ".intercalate (args.map (·.show argNames)) ++ ")"
+
+def Def.show (d : Def) (name : String) : String :=
+  let argNamesList := mkList d.arity λ i => String.ofList [.ofNat # 97 + i]
+  let argNames := .mk argNamesList
+  let argsStr := if d.arity = 0 then "" else
+    "(" ++ ", ".intercalate argNamesList ++ ")"
+  name ++ argsStr ++ " := " ++ d.expr.show argNames
+
+def ProgInfo.showWF {prog : Prog} [info : ProgInfo prog] : String :=
+  if !info.has_model then "no model"
+  else if !info.has_unique_model then "multiple models"
+  else "unique model"
+
+def Prog.show (prog : Prog) [info : ProgInfo prog] : String :=
+  let defs := "\n".intercalate # info.defNames.map # λ name =>
+    "".intercalate (List.replicate 2 " ") ++ (prog.def name).show name
+  "".intercalate ["program ", info.name, " -- ", info.showWF, "\n", defs]
